\documentclass[14 pt]{extarticle}

	\usepackage[frenchb]{babel}
	\usepackage[utf8]{inputenc}  
	\usepackage[T1]{fontenc}
	\usepackage{amssymb}
	\usepackage[mathscr]{euscript}
	\usepackage{stmaryrd}
	\usepackage{amsmath}
	\usepackage{tikz}
	\usepackage[all,cmtip]{xy}
	\usepackage{amsthm}
	\usepackage{varioref}
	\usepackage{geometry}
	\geometry{a4paper}
	\usepackage{lmodern}
	\usepackage{hyperref}
	\usepackage{array}
	 \usepackage{fancyhdr}
	 \usepackage{float}
\renewcommand{\theenumi}{\alph{enumi})}
	\pagestyle{fancy}
	\theoremstyle{plain}
\newcommand{\exo}[8]{
 \ \\ \ \\
 Nom : \ldots\ldots\ldots\ldots\ldots\ldots\ldots\ldots\ldots Prénom : \ldots\ldots\ldots \\ 
 Calculez :\\ \ \\ 
 \[ (- (#5 \times x +   =   \] 
 \[ (-3)^{-#6} = \] 
 \[ #7^2 = \]
 \[ \sqrt{#8} = \]
  }
	\fancyfoot[C]{} 
	\fancyhead[L]{}
	\fancyhead[R]{}\geometry{
 a4paper,
 total={170mm,257mm},
 left=20mm,
 top=20mm,
 }
	
	
	\title{Interrogation chapitre 5}
	\date{}
	\begin{document}
 \ \\ \ \\
 Nom : \ldots\ldots\ldots\ldots\ldots\ldots\ldots\ldots\ldots Prénom : \ldots\ldots\ldots \\ 
Développez et réduire :

 \[ (x^2 + 4) \times x = \]
 \[ (y+1)\times 6 - (3 + y) \times 2 = \]
 Convertir : 
 \[ 14 \text{ L} = \ldots\ldots\ldots\ldots \text{cm}^3\]
 \[ 24,31 \text{m}^3 = \ldots\ldots\ldots\ldots \text{L}\]
 
 \hrule
 \ \\ \ \\
 Nom : \ldots\ldots\ldots\ldots\ldots\ldots\ldots\ldots\ldots Prénom : \ldots\ldots\ldots \\ 
Développez et réduire :

 \[ (1 - y^2) \times y = \]
 \[ (x-1)\times 6 - (3 + x) \times 3 = \]
 Convertir : 
 \[ 54,12 \text{ cL} = \ldots\ldots\ldots \text{cm}^3\]
 \[ 965,12\text{mm}^3 = \ldots\ldots\ldots \text{L}\]
 
 \hrule
 \ \\ \ \\
 Nom : \ldots\ldots\ldots\ldots\ldots\ldots\ldots\ldots\ldots Prénom : \ldots\ldots\ldots \\ 
Développez et réduire :

 \[ (x^2 + x - 1) \times x = \]
 \[ (a-2)\times 3 - (2 +a) \times 2  = \]
 Convertir : 
 \[ 1543 \text{ L} = \ldots\ldots\ldots \text{m}^3\]
 \[ 546,124 \text{dm}^3 = \ldots\ldots\ldots \text{mL}\]
 
 \hrule
 \ \\ \ \\
 Nom : \ldots\ldots\ldots\ldots\ldots\ldots\ldots\ldots\ldots Prénom : \ldots\ldots\ldots \\ 
Développez et réduire :

 \[ (x^2 - 4x - 1) \times x = \]
 \[ (a+3)\times 4 - (3 + a) \times 2 = \]
 Convertir : 
 \[ 765,12 \text{cL} = \ldots\ldots\ldots \text{dm}^3\]
 \[ 78,124 \text{m}^3 = \ldots\ldots\ldots \text{L}\]
 
 \hrule
 
 
 
 	\end{document}
